http://atomurl.net/math/
https://ondiz.github.io/cursoLatex/Contenido/05.Ecuaciones.html

      %  \begin{equation}
      %      \left({\theta }_1,{\theta }_2,{\theta }_3\right)\ \to %E_0(x_0,y_0,z_0)\
      %  \end{equation}
      
      % ecuacioens en parrafos $...$
      $({\theta }_1,{\theta }_2,{\theta }_3)$
      
      
      % alinear ecuacioens con = 
          \begin{align}
        \phantom{i + j + k}
         &
         \begin{aligned}
            \mathllap{a} & = b + c + d\\ &\qquad + e + f + g + x + y + z
         \end{aligned}\\
         &
         \begin{aligned}
            \mathllap{i + j + k} & = l + m + n\\ &\qquad + o + p + q
         \end{aligned}
    \end{align}
    
    \begin{align}
\begin{split}\label{eq:1}
    a ={}& b + c + d\\
         & + e + f + g
\end{split}\\
\begin{split}\label{eq:2}
    k ={}& l + m + n + m + n + m + n\\
         & + o + p + q
\end{split}\\
    r ={}& s + t (u + v + w)\label{eq:3}
\end{align}
    
    \begin{align}
\begin{split}\label{eq:cap4_eq_3}
    E_0\left(x_0,y_0,z_0\right)& ={} \left(a_1z+\ b_1,a_2z+\ b_2,z\right)\\
         & ={} \left(a_1z+\ b_1,a_2z+\ b_2,\frac{-B-\ \sqrt{\left(B^2\right)-\left(4AC\right)}}{2*A}\right)\\
\end{split}\\
\end{align}
    
    
       \begin{align}
        z={}& \frac{-B\ \pm \ \sqrt{\left(B^2\right)-(4AC)}}{2*A} 
        \label{eq:cap4_eq_4} \\
        A={}& {a_1}^2+{a_2}^2+1
        \label{eq:cap4_eq_5} \\
        B={}&  2\left(a_1(b_1-x_1)+a_2(b_2-y_1)-z_1\right)
        \label{eq:cap4_eq_6} \\
        C={}& ({(b_1-x_1)}^2+{(b_2-y_1)}^2+{z_1}^2- {r_e}^2) 
        \label{eq:cap4_eq_7} \\
        a_1={}& \frac{\left(z_2-z_1\right)\left(y_3-y_1\right)-\left(z_3-z_1\right)\left(y_2-y_1\right)}{d} 
        \label{eq:cap4_eq_8} \\
        b_1={}& \left(\frac{1}{2*(-d)}\right)*\left(\left(w_2 - w_1\right)\left(y_3-y_1\right)-\left(w_3 - w_1\right)\left(y_2-y_1\right)\right)
        \label{eq:cap4_eq_9} \\
        a_2={}& \frac{-1}{d}*\left[\left(z_2-z_1\right)x_3-(z_3-z_1)x_2+(z_3-z_2)x_1\right]
        \label{eq:cap4_eq_10} \\
        b_2={}& \frac{1}{2d}*[\left(w_2-w_1\right)x_3-\left(w_3-w_1\right)x_2+\left(w_3-w_2)\right)x_1
        \label{eq:cap4_eq_11} \\
        d={}& \left(y_2- y_1\right)x_3-\left(y_3-y_1\right)x_2- \left(y_2-y_3\right)x_1
        \label{eq:cap4_eq_12} \\
        w_i={}& {x_i}^2+{y_i}^2 +{z_i}^2
        \label{eq:cap4_eq_13} 
    \end{align}
    
        \begin{align}
    \begin{split}
            E_0\left(x_0,y_0,z_0\right)& ={} \left(a_1z+\ b_1,a_2z+\ b_2,z\right)\\
                 & ={} \left(a_1z+\ b_1,a_2z+\ b_2,\frac{-B-\ \sqrt{\left(B^2\right)-\left(4AC\right)}}{2*A}\right)\\
    \end{split}
    \label{eq:cap4_eq_3}
    \end{align}
    